%!TEX program = xelatex
\documentclass[10pt, compress, handout]{beamer}
\usepackage[titleprogressbar]{../../cls/beamerthemem}

\usepackage{booktabs}
\usepackage[scale=2]{ccicons}
\usepackage{minted}

\usepgfplotslibrary{dateplot}

\usemintedstyle{trac}

\setbeamertemplate{caption}[numbered]
\setbeamertemplate{theorems}[numbered]
\newtheorem{crl}{Corollary}[theorem]
\newtheorem*{solution*}{Solution}

\usepackage{algorithm}
\usepackage[noend]{algpseudocode}

\usepackage{version}
\excludeversion{proof}
\excludeversion{solution*}

\usepackage{mathtools}
\usepackage{multicol}
\usepackage{qtree}

\makeatletter
\def\old@comma{,}
\catcode`\,=13
\def,{%
	\ifmmode%
	\old@comma\discretionary{}{}{}%
	\else%
	\old@comma%
	\fi%
}
\makeatother

\title{CSCI 3190 Tutorial of Week 10}
\subtitle{Traversal}
\author{LI Haocheng}
\institute{Department of Computer Science and Engineering}

\begin{document}

\maketitle

\begin{frame}[fragile]
	\frametitle{Expression}
	\begin{columns}
		\begin{column}{.6\linewidth}
			\onslide<1->\begin{example}
				\begin{enumerate}
					\item Represent the expression $((x + 2) \uparrow 3) \cdot (y - (3 + x)) - 5$ using a binary tree.
					\item Write this expression in prefix notation.
					\item Write this expression in postfix notation.
					\item Write this expression in infix notation.
				\end{enumerate}
			\end{example}
			\onslide<2>\begin{solution*}
				\begin{enumerate}
					\item $-\ \cdot\ \uparrow\ +\ x\ 2\ 3\ -\ y\ +\ 3\ x\ 5$
					\item $x\ 2\ +\ 3\ \uparrow\ y\ 3\ x\ +\ -\ \cdot\ 5\ -$
					\item $x\ +\ 2\ \uparrow\ 3\ \cdot\ y\ -\ 3\ +\ x\ -\ 5$
				\end{enumerate}
			\end{solution*}
		\end{column}
		\onslide<2>\begin{column}{.4\linewidth}
			\begin{solution*}
				\begin{figure}
					\centering
					$\Tree [.- [.\(\cdot\) [.\(\uparrow\) [.+ x 2 ] 3 ] [.- y [.+ 3 x ] ] ] 5 ]$
					\caption{A Rooted Tree $T$}
					\label{f-11-3-e16}
				\end{figure}
			\end{solution*}
		\end{column}
	\end{columns}
\end{frame}

\begin{frame}[fragile]
	\frametitle{Construction}
	\begin{columns}
		\begin{column}{.6\linewidth}
			\onslide<1->\begin{example}
				Construct the ordered rooted tree whose preorder traversal is $a, b, f, c, g, h, i, d, e, j, k, l$, where $a$ has four children, $c$ has three children, $j$ has two children, $b$ and $e$ have one child each, and all other vertices are leaves.
			\end{example}
		\end{column}
		\onslide<2>\begin{column}{.4\linewidth}
			\begin{solution*}
				\begin{figure}
					\centering
					$\Tree [.a [.b f ] [.c g h i ] d [.e [.j k l ] ] ]$
					\caption{A Rooted Tree $T$}
					\label{f-11-3-e25}
				\end{figure}
			\end{solution*}
		\end{column}
	\end{columns}
\end{frame}

\begin{frame}[fragile]
	\frametitle{Complexity}
	\onslide<1->\begin{example}
		Show the following:\begin{enumerate}[(a)]
			\item $3n^2 + 5n + 10 = O(n^2)$
		\end{enumerate}
	\end{example}
	\onslide<2>\begin{proof}
		\begin{enumerate}[(a)]
			\item \begin{description}
				\item[Method 1] $\exists c = 4, \exists N = 6$, such that $\forall n > N, 3n^2 + 5n + 10 < 4n^2$.
				\item[Method 2] Since $3 + \frac{5}{n} + \frac{10}{n^2} = O(1)$ and $n^2 = O(n^2)$, $3n^2 + 5n + 10 = O(n^2)$.
			\end{description}
		\end{enumerate}
	\end{proof}
\end{frame}

\begin{frame}[fragile]
	\frametitle{Complexity}
	\onslide<1->\begin{example}
		Show the following:\begin{enumerate}[(b)]
			\item $100 \log_2 n = O(n)$
		\end{enumerate}
	\end{example}
	\onslide<2>\begin{proof}
		\begin{enumerate}[(b)]
			\item \begin{description}
				\item[Method 1] Since $100 = O(1)$ and $\log_2 n = O(n)$, $100\log_2 n = O(n)$.
				\item[Method 2] \begin{align}
				& \lim\limits_{n \rightarrow \infty} \frac{100\log_2 n}{n}\\
				= & \frac{100}{\ln 2} \lim\limits_{n \rightarrow \infty} \frac{1}{n}\\
				= & 0
				\end{align}
			\end{description}
		\end{enumerate}
	\end{proof}
\end{frame}

\begin{frame}[fragile]
	\frametitle{Complexity}
	\onslide<1->\begin{example}
		Show the following:\begin{enumerate}[(a)]
			\setcounter{enumi}{2}
			\item $n! = O(n^n)$
			\item $2^n = O(n!)$
		\end{enumerate}
	\end{example}
	\onslide<2>\begin{proof}
		\begin{enumerate}[(a)]
			\setcounter{enumi}{2}
			\item $n! = \Pi_{i = 1}^n i \le \Pi_{i = 1}^n n = n^n$.
			\item $\exists c = 2, \exists N = 1$, such that $\forall n > N, 2^n = \Pi_{i = 1}^n 2 = 2 \Pi_{i = 2}^n 2 \le 2 \Pi_{i = 2}^n i = 2(n!)$.
		\end{enumerate}
	\end{proof}
\end{frame}

\plain{Questions?}

\end{document}
